examples/CCS/ExperimentalScript.sml
@@ -1,0 +1,70 @@
+(* ========================================================================== *)
+(* FILE          : ExperimentalScript.sml                                     *)
+(* DESCRIPTION   : Experimental and variant definitions                       *)
+(*                                                                            *)
+(* COPYRIGHTS    : 2023-2024 Australian National University (Chun Tian)       *)
+(******************************************************************************)
+
+open HolKernel Parse boolLib bossLib;
+
+open combinTheory pred_setTheory relationTheory pairTheory sumTheory listTheory
+     arithmeticTheory stringTheory;
+
+(* lambda theories *)
+open binderLib;
+
+(* local theories *)
+open CCSLib CCSTheory CCSSyntax CCSConv;
+open StrongEQTheory StrongEQLib StrongLawsTheory;
+open WeakEQTheory WeakEQLib WeakLawsTheory;
+open ObsCongrTheory ObsCongrLib ObsCongrLawsTheory;
+open CongruenceTheory CoarsestCongrTheory;
+open TraceTheory ExpansionTheory ContractionTheory;
+open BisimulationUptoTheory UniqueSolutionsTheory;
+(* open MultivariateTheory; *)
+
+val _ = new_theory "Experimental";
+
+(******************************************************************************)
+(*                                                                            *)
+(*         Variants of the transition relation (including coinductive)        *)
+(*                                                                            *)
+(******************************************************************************)
+
+(* coTRANS is the coinductive version of oTRANS with identical input rules *)
+CoInductive coTRANS :
+    (!E u.                             coTRANS (prefix u E) u E) /\         (* PREFIX *)
+    (!E u E1 E'.    coTRANS E u E1 ==> coTRANS (sum E E') u E1) /\          (* SUM1 *)
+    (!E u E1 E'.    coTRANS E u E1 ==> coTRANS (sum E' E) u E1) /\          (* SUM2 *)
+    (!E u E1 E'.    coTRANS E u E1 ==> coTRANS (par E E') u (par E1 E')) /\ (* PAR1 *)
+    (!E u E1 E'.    coTRANS E u E1 ==> coTRANS (par E' E) u (par E' E1)) /\ (* PAR2 *)
+    (!E l E1 E' E2. coTRANS E (label l) E1 /\ coTRANS E' (label (COMPL l)) E2
+                ==> coTRANS (par E E') tau (par E1 E2)) /\                  (* PAR3 *)
+    (!E u E' l L.   coTRANS E u E' /\ ((u = tau) \/
+                                     ((u = label l) /\ l NOTIN L /\ (COMPL l) NOTIN L))
+                ==> coTRANS (restr L E) u (restr L E')) /\                  (* RESTR *)
+    (!E u E' rf.    coTRANS E u E'
+                ==> coTRANS (relab E rf) (relabel rf u) (relab E' rf)) /\   (* RELABELING *)
+    (!E u X E1.     coTRANS (CCS_Subst E (rec X E) X) u E1
+                ==> coTRANS (rec X E) u E1)                                 (* REC *)
+End
+
+(* The rules for the transition relation TRANS as individual theorems. *)
+val [coPREFIX, coSUM1, coSUM2, coPAR1, coPAR2, coPAR3, coRESTR, coRELABELING, coREC] =
+    map save_thm
+        (combine (["coPREFIX", "coSUM1", "coSUM2", "coPAR1", "coPAR2", "coPAR3",
+                   "coRESTR", "coRELABELING", "coREC"],
+                  CONJUNCTS coTRANS_rules));
+
+(* Use SUB instead of CCS_Subst *)
+Theorem coREC' = REWRITE_RULE [CCS_Subst] coREC
+
+val _ = export_theory ();
+val _ = html_theory "Experimental";
+
+(* Bibliography:
+
+ [1] Milner, Robin. Communication and concurrency. Prentice hall, 1989.
+ [2] Gorrieri, R., Versari, C.: Introduction to Concurrency Theory. Springer (2015).
+
+ *)
